specs/lemmas/Spec.P256.Lemmas.fst
@@ -7,14 +7,6 @@ module M = Lib.NatMod
 
 #set-options "--z3rlimit 50 --ifuel 0 --fuel 0"
 
-let lemma_proj_aff_id p = admit()
-
-let lemma_aff_is_point_at_inf p =
-  prime_lemma ();
-  let (px, py, pz) = p in
-  M.lemma_div_mod_prime_is_zero #prime px pz;
-  M.lemma_div_mod_prime_is_zero #prime py pz
-
 let to_aff_point_at_infinity_lemma () = admit()
 
 let to_aff_point_add_lemma p q = admit()
