specs/ecc/Spec.EC.Projective.Lemmas.fst
@@ -1,0 +1,26 @@
+module Spec.EC.Projective.Lemmas
+
+open FStar.Mul
+
+module M = Lib.NatMod
+
+open Spec.EC.Projective
+
+#set-options "--z3rlimit 50 --fuel 0 --ifuel 0"
+
+let lemma_aff_is_point_at_inf k p =
+  k.prime_lemma ();
+  let (px, py, pz) = p in
+  M.lemma_div_mod_prime_is_zero #prime px pz;
+  M.lemma_div_mod_prime_is_zero #prime py pz
+
+
+let lemma_proj_aff_id k p =
+  let (px, py) = p in
+  let (pX, pY, pZ) = to_proj_point k p in
+  assert (pX = px /\ pY = pY /\ pZ = 1);
+  let (rx, ry) = to_aff_point k (pX, pY, pZ) in
+  assert (rx = fmul k pX (finv k pZ) /\ ry = fmul k pY (finv k pZ));
+  M.lemma_div_mod_prime_one #prime pX;
+  M.lemma_div_mod_prime_one #prime pY;
+  assert (rx = pX /\ ry = pY)
