specs/ecc/Spec.EC.Projective.Lemmas.fsti
@@ -1,0 +1,14 @@
+module Spec.EC.Projective.Lemmas
+
+open FStar.Mul
+open Spec.EC.Projective
+
+#set-options "--z3rlimit 50 --fuel 0 --ifuel 0"
+
+val lemma_aff_is_point_at_inf: k:curve -> p:proj_point k ->
+  Lemma (let px, py, pz = p in
+    is_aff_point_at_inf k (to_aff_point k p) == (pz = 0 || (px = 0 && py = 0)))
+
+
+val lemma_proj_aff_id (k:curve) (p:aff_point k) :
+  Lemma (to_aff_point k (to_proj_point k p) == p)
