specs/ecc/Spec.EC.Projective.fst
@@ -1,0 +1,29 @@
+module Spec.EC.Projective
+
+open FStar.Mul
+
+include Spec.EC
+
+#set-options "--z3rlimit 50 --fuel 0 --ifuel 0"
+
+let proj_point (k:curve) =
+  p:tuple3 nat nat nat{let (px, py, pz) = p in px < prime /\ py < prime /\ pz < prime}
+
+
+let point_at_inf (k:curve) : proj_point k =
+  (zero k, one k, zero k)
+
+let is_point_at_inf (k:curve) (p:proj_point k) =
+  let (_, _, z) = p in z = zero k
+
+
+let to_proj_point (k:curve) (p:aff_point k) : proj_point k =
+  let (x, y) = p in (x, y, one k)
+
+let to_aff_point (k:curve) (p:proj_point k) : aff_point k =
+  // if is_proj_point_at_inf p then aff_point_at_inf
+  let (px, py, pz) = p in
+  let zinv = finv k pz in
+  let x = fmul k px zinv in
+  let y = fmul k py zinv in
+  (x, y)
