specs/lemmas/Spec.K256.Lemmas.fsti
@@ -4,19 +4,10 @@ open FStar.Mul
 
 open Spec.K256.PointOps
 
-module EC = Spec.EC
+module EC = Spec.EC.Projective
 module LM = Lib.NatMod
 
 #set-options "--z3rlimit 50 --ifuel 0 --fuel 0"
-
-val lemma_aff_is_point_at_inf: p:proj_point ->
-  Lemma (let px, py, pz = p in
-    EC.is_aff_point_at_inf k256 (to_aff_point p) == (pz = 0 || (px = 0 && py = 0)))
-
-
-val lemma_proj_aff_id (p:EC.aff_point k256) :
-  Lemma (to_aff_point (to_proj_point p) == p)
-
 
 // TODO: mv to Spec.EC
 val aff_point_negate_lemma (p:EC.aff_point k256) :
@@ -24,22 +15,25 @@ val aff_point_negate_lemma (p:EC.aff_point k256) :
 
 
 val to_aff_point_at_infinity_lemma: unit ->
-  Lemma (to_aff_point point_at_inf == EC.aff_point_at_inf k256)
+  Lemma (EC.to_aff_point k256 (EC.point_at_inf k256) == EC.aff_point_at_inf k256)
 
 
-val to_aff_point_add_lemma (p q:proj_point) :
-  Lemma (to_aff_point (point_add p q) == EC.aff_point_add k256 (to_aff_point p) (to_aff_point q))
+val to_aff_point_add_lemma (p q:EC.proj_point k256) :
+  Lemma (EC.to_aff_point k256 (point_add p q) ==
+    EC.aff_point_add k256 (EC.to_aff_point k256 p) (EC.to_aff_point k256 q))
 
 
-val to_aff_point_double_lemma (p:proj_point) :
-  Lemma (to_aff_point (point_double p) == EC.aff_point_add k256 (to_aff_point p) (to_aff_point p))
+val to_aff_point_double_lemma (p:EC.proj_point k256) :
+  Lemma (EC.to_aff_point k256 (point_double p) ==
+    EC.aff_point_add k256 (EC.to_aff_point k256 p) (EC.to_aff_point k256 p))
 
 
-val to_aff_point_negate_lemma (p:proj_point) :
-  Lemma (to_aff_point (point_negate p) == aff_point_negate (to_aff_point p))
+val to_aff_point_negate_lemma (p:EC.proj_point k256) :
+  Lemma (EC.to_aff_point k256 (point_negate p) == aff_point_negate (EC.to_aff_point k256 p))
 
 
 // works when q < prime /\ prime < 2 * q
-val ecdsa_verify_avoid_finv: p:proj_point{not (is_proj_point_at_inf p)} -> r:nat{0 < r /\ r < q} ->
+val ecdsa_verify_avoid_finv: p:EC.proj_point k256{not (EC.is_point_at_inf k256 p)}
+  -> r:nat{0 < r /\ r < q} ->
   Lemma (let _X, _Y, _Z = p in
     (_X /% _Z % q = r) <==> ((r *% _Z = _X) || (r + q < prime && (r + q) *% _Z = _X)))
